\documentclass[14pt]{beamer}
\input{../../../beamer-preamble-2020}
\usetheme{default}
\usecolortheme{seahorse}

\title[] {Finding the Equation of a Line Given the Slope and a Point or Two Points}
\author{Jonathan R. Bacolod}
\institute[SHS]{Sauyo High School}
\date{}

\begin{document}
	\frame{\titlepage}
	
	\begin{frame}
		\frametitle{How to Find the Equation of a Line?}
		Use the formulae:
		\begin{enumerate}  
			\item Slope-intercept form: $ y = mx + b $
			\item \pause Point-slope form: $ y - y_1 = m(x - x_1) $
			\item \pause Two-point form: $  \dfrac{y - y_1}{y_2 - y_1} = \dfrac{x - x_1}{x_2 - x_1}$
		\end{enumerate}  
	\end{frame}

    \begin{frame}
    	\frametitle{How to Find the Equation of a Line Given the Slope and a Point?}
    	Use the point-slope form:  $ y - y_1 = m(x - x_1) $
    \end{frame}

    \begin{frame}
    	\frametitle{Example 1}
    	Find the equation of the line with a slope equal to $ 2 $ and passes through point $ (1, 3) $.
    	    	
    	\begin{TAB}(@, 1mm, 5mm)[2mm]{ll}{ccccccc}
    		\pause Given: $ m = 2 $,  & \pause $ (x_1, y_1) = (1, 3) $  \\
    		
    		\pause $ y - y_1 = m(x - x_1)  $  &  \\
    		
    		\pause $ y - 3 = 2(x - 1)  $ & \pause Substitution \\
    		
    		\pause $ y - 3 = 2x - 2  $ & \pause Distributive Property \\
    		
    		\pause $ y = 2x - 2 + 3 $ & \pause Addition Property \\
    		
    		\pause $ y = 2x + 1 $ & \pause Simplification \\
    		& \\
    	\end{TAB}
  
      $ \therefore $ the equation of the line is $ y = 2x + 1 $.
    \end{frame}

    \begin{frame}
    	\frametitle{Example 2}
    	\footnotesize Find the equation of the line with a slope equal to $ \dfrac{2}{3} $ and contains the point $ (9, 7) $.
    	
    	\begin{TAB}(@, 1mm, 5mm)[2mm]{ll}{cccccc}
    		\pause Given: $ m = \dfrac{2}{3} $,  & \pause $ (x_1, y_1) = (9, 7) $  \\
    		
    		\pause $ y - y_1 = m(x - x_1)  $  &  \\
    		
    		\pause $ y - 7 = \dfrac{2}{3}(x - 9)  $ & \pause Substitution \\
    		
    		\pause $ y - 7 = \dfrac{2}{3}x - 6  $ & \pause Distributive Property \\
    		
    		\pause $ y = \dfrac{2}{3}x - 6 + 7 $ & \pause Addition Property \\
    		
    		\pause $ y = \dfrac{2}{3}x + 1 $ &  Simplification \\
%    		& \\
    	\end{TAB}
    	
    	$ \therefore $ the equation of the line is $ y = \dfrac{2}{3}x + 1 $.
    \end{frame}

    \begin{frame}
    	\frametitle{Example 3}
    	Find the equation of the line parallel to $ y = 3x - 2 $ and passes through point $ (1, -1) $.
    	
    	\begin{TAB}(@, 1mm, 5mm)[2mm]{ll}{ccccccc}
    		\pause Given: $ m = 3 $,  & \pause $ (x_1, y_1) = (1, -1) $  \\
    		
    		\pause $ y - y_1 = m(x - x_1)  $  &  \\
    		
    		\pause $ y - (-1) = 3(x - 1)  $ & \pause Substitution \\
    		
    		\pause $ y + 1 = 3x - 3  $ & \pause Distributive Property \\
    		
    		\pause $ y = 3x - 3 - 1 $ & \pause Subtraction Property \\
    		
    		\pause $ y = 3x - 4 $ & \pause Simplification \\
    		& \\
    	\end{TAB}
    	
    	$ \therefore $ the equation of the line is $ y = 3x - 4 $.
    \end{frame}

    \begin{frame}
    	\frametitle{How to Find the Equation of a Line Given Two Points?}
    	Use the two-point form: $  \dfrac{y - y_1}{y_2 - y_1} = \dfrac{x - x_1}{x_2 - x_1}$
    \end{frame}

    \begin{frame}
    	\frametitle{Example 1}
    	Write the equation of the line containing $ (1, 1) $ and $ (3, -1) $. 
    	
    \lcmtwobytwolineone{-2}{(2)}{(-1)}
    \lcmtwobytwolinetwo{2}{(2)}{}
    \lcmtwobytwolinethree{2}{-1}{-2}
    
       	\begin{TAB}(@, 1mm, 5mm)[2mm]{ll}{cccccc}
    		\pause Given: $ (x_1, y_1) = (1, 1)  $,  & \pause $ (x_2, y_2) = (3, -1) $  \\
    		
    		\pause $ \dfrac{y - y_1}{y_2 - y_1} = \dfrac{x - x_1}{x_2 - x_1}  $  &  \\
    		
    		\pause $ \dfrac{y - 1}{-1 - 1} = \dfrac{x - 1}{3 - 1}  $ & \pause Substitution \\
    		
    		\pause $ \dfrac{y - 1}{-2} = \dfrac{x - 1}{2} $ & \pause Simplification \\
    		
    	    \only<7-19>{\footnotesize \lcmtwobytwo{1}{0.1} \normalsize} \only<20->{$ -2 \left[\dfrac{y - 1}{-2} \right] = -2\left[\dfrac{x - 1}{2} \right] $} & \only<21->{ Multiplication} \\
    		& \\
    	\end{TAB}
    \end{frame}

    \begin{frame}
    	\frametitle{Example 1}
    	\begin{TAB}(@, 1mm, 5mm)[2mm]{ll}{ccccc}
    	  $ -2 \left[\dfrac{y - 1}{-2} \right] = -2\left[\dfrac{x - 1}{2} \right] $ &  Multiplication \\
    		
    		\pause $ y - 1 = -x + 1 $ &\pause Distributive Property \\
    		
    		\pause $ y = -x + 1 + 1 $ &\pause Addition Property \\
    		
    		\pause $ y = -x + 2 $ & \pause Simplification \\
    		& \\
    	\end{TAB}
    	
    	$ \therefore $ the equation of the line is $ y = -x + 2 $.
    \end{frame}
    
    \begin{frame}
    	\frametitle{Example 2}
    	Write the equation of the line that passes through $ (2, 4) $ and whose x-intercept is $ 1 $. 
    	
    	\lcmtwobytwolineone{-1}{(-1)}{}
    	\lcmtwobytwolinetwo{-4}{(-1)}{(2^2)}
    	\lcmtwobytwolinethree{-1}{2^2}{-4}
    	
    	\begin{TAB}(@, 1mm, 5mm)[2mm]{ll}{cccccc}
    		\pause Given: $ (x_1, y_1) = (2, 4)  $,  & \pause $ (x_2, y_2) = (1, 0) $  \\
    		
    		\pause $ \dfrac{y - y_1}{y_2 - y_1} = \dfrac{x - x_1}{x_2 - x_1}  $  &  \\
    		
    		\pause $ \dfrac{y - 4}{0 - 4} = \dfrac{x - 2}{1 - 2}  $ & \pause Substitution \\
    		
    		\pause $ \dfrac{y - 4}{-4} = \dfrac{x - 2}{-1} $ & \pause Simplification \\
    		
    		 \only<7-19>{\footnotesize \lcmtwobytwo{1}{0.1} \normalsize} \only<20->{$ -4 \left[\dfrac{y - 4}{-4} \right] = -4\left[\dfrac{x - 2}{-1} \right] $} & \only<21->{ Multiplication} \\
    		    		& \\
    	\end{TAB}
    \end{frame}

    \begin{frame}
	\frametitle{Example 2}
	
	\begin{TAB}(@, 1mm, 5mm)[2mm]{ll}{ccccc}
		$ -4 \left[\dfrac{y - 4}{-4} \right] = -4\left[\dfrac{x - 2}{-1} \right] $ &  Multiplication \\
		
		\pause $ y - 4 = 4x - 8 $ & \pause Distributive Property \\
		
		\pause $ y = 4x - 8 + 4 $ & \pause Addition Property \\
		
		\pause $ y = 4x - 4 $ & Simplification \\
		    		& \\
	\end{TAB}
	
	$ \therefore $ the equation of the line is $ y = 4x - 4 $.
\end{frame}


    \begin{frame}
    	\frametitle{Example 3}
    	Write the equation of the line passing through the points $ (-7, -1) $ and $ (1, -3) $. 
    	
    	\lcmtwobytwolineone{-2}{(2)}{(-1)}
    	\lcmtwobytwolinetwo{8}{(2^3)}{}
    	\lcmtwobytwolinethree{2^3}{-1}{-8}
    	
    	\begin{TAB}(@, 1mm, 5mm)[2mm]{ll}{cccccc}
    		\pause Given: $ (x_1, y_1) = (-7, -1)  $,  & \pause $ (x_2, y_2) = (1, -3) $  \\
    		
    		\pause $ \dfrac{y - y_1}{y_2 - y_1} = \dfrac{x - x_1}{x_2 - x_1}  $  &  \\
    		
    		\pause $ \dfrac{y - (-1)}{-3 - (-1)} = \dfrac{x - (-7)}{1 - (-7)}  $ & \pause Substitution \\
    		
    		\pause $ \dfrac{y + 1}{-2} = \dfrac{x + 7}{8} $ & \pause Simplification \\
    		
    		\only<7-19>{\footnotesize \lcmtwobytwo{1}{0.1} \normalsize} \only<20->{$ -8 \left[\dfrac{y + 1}{-2} \right] = -8\left[\dfrac{x + 7}{8} \right] $} & \only<21->{ Multiplication} \\
    		    		& \\
    	\end{TAB}
    \end{frame}

    \begin{frame}
	\frametitle{Example 3}
	\begin{TAB}(@, 1mm, 5mm)[2mm]{ll}{cccccc}
		$ -8 \left[\dfrac{y + 1}{-2} \right] = -8\left[\dfrac{x + 7}{8} \right] $ &  Multiplication \\
		
		\pause $ 4y + 4 = -x - 7 $ & \pause Distributive Property \\
		
		\pause $ 4y = -x - 7 - 4 $ & \pause Subtraction Property \\
		
		\pause $ 4y = -x - 11 $ & \pause Simplification \\
		
		\pause $ \dfrac{4y}{4} = \dfrac{-x}{4} - \dfrac{11}{4} $ & \pause Division Property \\
		
		\pause $ y = -\dfrac{1}{4}x - \dfrac{11}{4} $ & Simplification \\
	\end{TAB}
	
	$ \therefore $ the equation of the line is $ y = -\dfrac{1}{4}x - \dfrac{11}{4} $.
\end{frame}

\begin{frame}
	\frametitle{How to Find the Equation of a Line?}
	Use the formulae:
	\begin{enumerate}  
		\item Slope-intercept form: $ y = mx + b $
		\item \pause Point-slope form: $ y - y_1 = m(x - x_1) $
		\item \pause Two-point form: $  \dfrac{y - y_1}{y_2 - y_1} = \dfrac{x - x_1}{x_2 - x_1}$
	\end{enumerate}  
\end{frame}

\begin{frame}
	\frametitle{How to Find the Equation of a Line Given the Slope and a Point?}
	Use the point-slope form:  $ y - y_1 = m(x - x_1) $
\end{frame}

    \begin{frame}
	\frametitle{How to Find the Equation of a Line Given Two Points?}
	Use the two-point form: $  \dfrac{y - y_1}{y_2 - y_1} = \dfrac{x - x_1}{x_2 - x_1}$
\end{frame}

    \begin{frame}
    	\begin{center}
    		\textbf{\LARGE Thank you for watching.}
    	\end{center}
    \end{frame}
	
\end{document}